Improvement (again) in printing failure handling
There are situations where the injected print code for "val _ = _ : _" may fail
to type check, e.g. if the necessary pp_X functions have somehow been shadowed
and got the wrong type, or maybe other ways.

To (yet again) try to handle this better, type check each val-print declaration
in isolation, handling the type error by replacing just that declaration with
a safer version from a range of 3 progressively safer options.

This should provide a little more information to the user in this case, rather
than a single error and the loss of information for the whole block.

compiler/printing/printTweaksScript.sml
@@ -16,14 +16,29 @@ Definition print_failure_message_def:
 End
 
 Definition add_err_message_def:
-  add_err_message s decs tn ienv inf_st =
+  add_err_message s decs_ext st =
   (* something's gone wrong, try to add a message *)
+  let (tn, ienv, inf_st) = st in
   let pmsg = [print_failure_message s] in
   case infer_ds ienv pmsg inf_st of
-  (Success msg_ienv, inf_st2) =>
-      (Success (decs ++ pmsg, (tn, extend_dec_ienv msg_ienv ienv, inf_st2)))
+  | (Success msg_ienv, inf_st2) =>
+        (pmsg ++ decs_ext, (tn, extend_dec_ienv msg_ienv ienv, inf_st2))
   (* if even that fails, skip it *)
-  | (Failure _, _) => Success (decs, (tn, ienv, inf_st))
+  | (Failure _, _) => (decs_ext, (tn, ienv, inf_st))
+End
+
+Definition add_print_from_opts_def:
+  add_print_from_opts nm [] (decs_ext, st) =
+  add_err_message (strlit "exhausted print options for " ^ strlit nm) decs_ext st /\
+  add_print_from_opts nm (print_opt :: xs) (decs_ext, st) =
+  let (tn, ienv, inf_st) = st in
+  case infer_ds ienv [print_opt] inf_st of
+  | (Success ienv2, inf_st2) =>
+        (print_opt :: decs_ext, (tn, extend_dec_ienv ienv2 ienv, inf_st2))
+  | (Failure x, _) =>
+  let (decs_ext, st) = add_err_message
+        (strlit "adding val pretty-print: " ^ SND x) decs_ext st in
+  add_print_from_opts nm xs (decs_ext, st)
 End
 
 Definition add_print_features_def:
@@ -34,17 +49,16 @@ Definition add_print_features_def:
   (Success decs_ienv, inf_st) =>
   let (prints, tn2) = val_prints tn ienv decs_ienv in
   let ienv2 = extend_dec_ienv decs_ienv ienv in
-  (case infer_ds ienv2 prints inf_st of
-  (Success prints_ienv, inf_st2) =>
-      (Success (decs2 ++ prints, (tn2, extend_dec_ienv prints_ienv ienv2, inf_st2)))
-  | (Failure x, _) => add_err_message (strlit "adding val pretty-prints: " ^ SND x)
-        decs2 tn2 ienv2 inf_st
-  )
+  let (print_decs_ext, st) = FOLDR (\(nm, opts). add_print_from_opts nm opts)
+        ([], (tn2, ienv2, inf_st)) prints in
+  (Success (decs2 ++ REVERSE print_decs_ext, st))
   | (Failure x, _) =>
   (* maybe the default pretty-printer decs are the problem *)
   (case infer_ds ienv decs (init_infer_state <| next_id := next_id |>) of
-  (Success ienv3, inf_st3) => add_err_message (strlit "adding type pp funs: " ^ SND x)
-        decs tn (extend_dec_ienv ienv3 ienv) inf_st3
+  (Success ienv3, inf_st3) =>
+  let (decs_ext, st) = add_err_message (strlit "adding type pp funs: " ^ SND x)
+        [] (tn, extend_dec_ienv ienv3 ienv, inf_st3) in
+  (Success (decs ++ REVERSE decs_ext, st))
   | (Failure x, _) => Failure x
   )
 End
@@ -96,19 +110,103 @@ Proof
   )
 QED
 
+Theorem add_err_message_infer:
+  add_err_message s decs_ext (tn, extend_dec_ienv ienv init_ienv, inf_st) =
+    (decs_ext2, st2) /\
+  infer_ds init_ienv (REVERSE decs_ext) init_inf_st = (Success ienv, inf_st) ==>
+  ?tn2 ienv_res inf_st2 ienv2.
+  st2 = (tn2, ienv_res, inf_st2) /\
+  infer_ds init_ienv (REVERSE decs_ext2) init_inf_st = (Success ienv2, inf_st2) /\
+  ienv_res = extend_dec_ienv ienv2 init_ienv
+Proof
+  simp [add_err_message_def]
+  \\ every_case_tac
+  \\ rw []
+  \\ simp [infer_ds_append]
+  \\ simp [extend_dec_ienv_def]
+QED
+
+Theorem add_print_from_opts_infer:
+  !opts decs_ext tn ienv inf_st decs_ext2 tn2 ienv_res inf_st2.
+  add_print_from_opts nm opts (decs_ext, (tn, extend_dec_ienv ienv init_ienv, inf_st)) =
+    (decs_ext2, st2) /\
+  infer_ds init_ienv (REVERSE decs_ext) init_inf_st = (Success ienv, inf_st) ==>
+  ?tn2 ienv_res inf_st2 ienv2.
+  st2 = (tn2, ienv_res, inf_st2) /\
+  infer_ds init_ienv (REVERSE decs_ext2) init_inf_st = (Success ienv2, inf_st2) /\
+  ienv_res = extend_dec_ienv ienv2 init_ienv
+Proof
+  Induct
+  \\ rw [add_print_from_opts_def]
+  >- (
+    drule_then drule add_err_message_infer
+    \\ rw [] \\ simp []
+  )
+  \\ every_case_tac
+  >- (
+    gvs []
+    \\ simp [infer_ds_append]
+    \\ simp [extend_dec_ienv_def]
+  )
+  >- (
+    rpt (pairarg_tac \\ fs [])
+    \\ drule_then drule add_err_message_infer
+    \\ rw []
+    \\ first_x_assum (drule_then drule)
+    \\ simp []
+  )
+QED
+
+Triviality fold_add_print_from_opts_infer:
+  !xs decs_ext tn ienv inf_st decs_ext2 st2 tn2 ienv_res inf_st2.
+  FOLDR (\(nm, opts). add_print_from_opts nm opts)
+    (decs_ext, (tn, extend_dec_ienv ienv init_ienv, inf_st)) xs =
+    (decs_ext2, st2) /\
+  infer_ds init_ienv (REVERSE decs_ext) init_inf_st = (Success ienv, inf_st) ==>
+  ?tn2 ienv_res inf_st2 ienv2.
+  st2 = (tn2, ienv_res, inf_st2) /\
+  infer_ds init_ienv (REVERSE decs_ext2) init_inf_st = (Success ienv2, inf_st2) /\
+  ienv_res = extend_dec_ienv ienv2 init_ienv
+Proof
+  Induct \\ rw [] \\ simp []
+  \\ rpt (pairarg_tac \\ fs [])
+  \\ qmatch_asmsub_abbrev_tac `add_print_from_opts _ _ tup`
+  \\ Cases_on `tup`
+  \\ gvs [markerTheory.Abbrev_def, Q.ISPEC `(_, _)` EQ_SYM_EQ]
+  \\ first_x_assum (drule_then drule)
+  \\ rw []
+  \\ drule_then drule add_print_from_opts_infer
+  \\ simp []
+QED
+
+Triviality extend_none:
+  extend_dec_ienv <|inf_v := nsEmpty; inf_c := nsEmpty; inf_t := nsEmpty|> ienv = ienv
+Proof
+  simp [extend_dec_ienv_def, inf_env_component_equality]
+QED
+
+Triviality fold_add_print_from_opts_infer2 =
+    Q.SPECL [`xs`, `[]`] fold_add_print_from_opts_infer
+    |> SIMP_RULE (srw_ss ()) [infer_d_def, st_ex_return_def, extend_none]
+
+Triviality add_err_message_infer2 = add_err_message_infer
+    |> Q.GENL [`decs_ext`, `ienv`, `inf_st`] |> Q.SPEC `[]`
+    |> SIMP_RULE (srw_ss ()) [infer_d_def, st_ex_return_def, extend_none]
+
 Theorem add_print_features_succ:
   add_print_features st decs = (infer$Success (decs2, st2)) ==>
   ?tn ienv next_id tn2 ienv2 inf_st2.
   st = (tn, ienv, next_id) /\ st2 = (tn2, extend_dec_ienv ienv2 ienv, inf_st2) /\
   infer_ds ienv decs2 (init_infer_state <| next_id := next_id |>) = (Success ienv2, inf_st2)
 Proof
-  fs [add_print_features_def, add_err_message_def]
+  fs [add_print_features_def]
   \\ rpt (pairarg_tac \\ fs [])
   \\ simp [pairTheory.pair_case_eq, exc_case_eq]
   \\ rw []
   \\ rpt (pairarg_tac \\ fs [])
-  \\ fs [pairTheory.pair_case_eq, exc_case_eq]
-  \\ rpt VAR_EQ_TAC
+  \\ gvs []
+  \\ (drule fold_add_print_from_opts_infer2 ORELSE drule add_err_message_infer2)
+  \\ rw []
   \\ simp [infer_ds_append]
   \\ simp [extend_dec_ienv_def]
 QED
